ITrees trans

theories/CTree/Logic/Entails.v
@@ -1,65 +1,35 @@
-From ExtLib Require Import
-  Structures.MonadWriter
-  Structures.Monads
-  Structures.MonadState
-  Data.Monads.StateMonad.
-
 From Coq Require Import
-  List
-  Basics
-  Fin
-  Relations.Relation_Definitions
   Classes.SetoidClass
+  Classes.Morphisms
   Classes.RelationPairs.
 
 From CTree Require Import
-  CTree.Core
-  CTree.Pred
-  CTree.Equ
-  CTree.SBisim
-  CTree.Trans
-  CTree.Logic.Trans
-  Logic.Semantics
-  Logic.Entails
   Logic.Kripke
-  Events.Writer.
+  Logic.Semantics
+  Logic.Congruence.
 
 Generalizable All Variables.
 
-Import Ctree CTreeNotations.
-Local Open Scope ctree_scope.
+Arguments CtlFormula: clear implicits.
 
-Section KripkeCTreeW.
-  Context {E W: Type}.
-  Local Open Scope ctl_scope.
-
-  (*| CTreeW is an interpreted tree, an automaton by indirection to [ctree_kripke] |*)
-  #[refine] Global Instance ctreeW_kripke: Kripke (ctreeW W) W :=
-    {|
-      ktrans X '(t, w) '(t', w') :=
-        ctree_kripke.(ktrans) (X:=X)
-                       (t, Some (Obs (Log w) tt))
-                       (t', Some (Obs (Log w') tt));
-      mequ X := @sbisim (writerE W) (writerE W) _ _ X X eq
-    |}.
-  Proof.
-    intros; now apply ctree_kripke.(ktrans_semiproper) with (t:=t) (s:=s).
-  Defined.
-
-End KripkeCTreeW.
-
-(*
-  - Uninterpreted ctree (observe uninterpreted events)
-    + ctree E X * opt E (from [ctree_kripke])
-  - Interpreterd (observe states)
-    + stateT W (ctree (writerE W))
-  - Interpreted (observe interpreted events)
-    + stateT Σ (ctree (writerE (Bar E)))
- *)
-Global Instance ctreeW_entails{W}: EntailsT (ctreeW W) W := {
-    KripkeM := @ctreeW_kripke W;
-    entails {X} (φ: CtlFormula W) (t: ctreeW W X) (w: W) :=
-      entails
-        (ctl_option (ctl_contramap (fun '(Obs (Log w) _) => w) φ))
-        t (Some (Obs (Log w) tt))
+Class EntailsT(M: Type -> Type)(W: Type) := {
+    KripkeM :: Kripke M W;
+    entails{X}(φ: CtlFormula W)(m: M X)(w: W): Prop
   }.
+Global Hint Mode EntailsT ! +: core.
+
+(* Entails instances for all the following.
+   Base entailsF is (M X * W).
+   - Uninterpreted ctree (observe uninterpreted events)
+     + ctree E X * opt E
+   - Interpreterd (observe states)
+     + stateT Σ (ctree (writerE Σ))
+   - Interpreted (observe interpreted events)
+     + stateT Σ (ctree (writerE (Bar E)))
+*)
+Global Instance EntailsT_id `{Kripke M W}: EntailsT M W :=
+  {
+    entails{X}(φ: CtlFormula W)(m: M X)(w: W) :=
+      entailsF φ (m, w)
+  }.
+
