theories/Logic/.#Kripke.v
@@ -1,1 +1,0 @@
-elefthei@nebuchadnezzar.6114:1701356333
